fairneris/fair_resources.v
@@ -167,6 +167,7 @@ Section model_state_interp.
   Context `{LM: LiveModel Λ M}.
   Context {Σ : gFunctors}.
   Context {fG: fairnessGS LM Σ}.
+  Context `{!invGS_gen HasNoLc Σ}.
 
   Notation Role := (M.(fmrole)).
 
@@ -214,17 +215,21 @@ Section model_state_interp.
              (fuel_map : gmap (locale Λ) (gmap Role nat)) :=
      ∀ ζ, ζ ∉ locales_of_list tp → fuel_map !! ζ = None.
 
-  Definition model_state_interp (tp: list $ expr Λ) (δ: LiveState Λ M): iProp Σ :=
+  Definition config_update_state : iProp Σ :=
+    ∀ m1 m2 cl fl, ⌜ LM.(lm_cfg_action) m1 cl = (fl, m2) ⌝ -∗ auth_model_is m1 ={⊤}=∗ auth_model_is m2.
+
+  Definition model_state_interp (tp: list $ expr Λ) (δ: LiveStateData Λ M): iProp Σ :=
+    □ config_update_state ∗
     ∃ fuel_map,
       ⌜ fuel_map_le fuel_map δ.(ls_map) ⌝ ∗
       ⌜ fuel_map_preserve_dead fuel_map (M.(live_roles) δ) ⌝ ∗
       ⌜ fuel_map_preserve_threadpool tp fuel_map ⌝ ∗
       auth_model_is δ ∗ auth_fuel_mapping_is fuel_map.
 
-  Lemma model_state_interp_tids_smaller δ tp :
+  Lemma model_state_interp_tids_smaller (δ : LiveState _ _) tp :
     model_state_interp tp δ -∗ ⌜ tids_smaller tp δ ⌝.
   Proof.
-    iIntros "(%m&[_ %Heq]&%&%Hbig&_)".
+    iIntros "(?&%m&[_ %Heq]&%&%Hbig&_)".
     iPureIntro.
     intros ζ Hin.
     assert (¬ (ζ ∉ locales_of_list tp)).
@@ -344,6 +349,7 @@ Section model_state_lemmas.
   Context `{EqDecision (expr Λ)}.
   Context {Σ : gFunctors}.
   Context {fG: fairnessGS LM Σ}.
+  Context `{!invGS_gen HasNoLc Σ}.
 
   Lemma update_model δ δ1 δ2:
     auth_model_is δ1 -∗ frag_model_is δ2 ==∗ auth_model_is δ ∗ frag_model_is δ.
@@ -365,7 +371,7 @@ Section model_state_lemmas.
   Lemma model_agree' δ1 s2 n:
     model_state_interp n δ1 -∗ frag_model_is s2 -∗ ⌜ ls_under δ1 = s2 ⌝.
   Proof.
-    iIntros "Hsi Hs2". iDestruct "Hsi" as (??) "(_&_&Hs1&_)".
+    iIntros "Hsi Hs2". iDestruct "Hsi" as "(?&%fm&?&_&_&Hs1&_)".
     iApply (model_agree with "Hs1 Hs2").
   Qed.
 
@@ -438,13 +444,12 @@ Section model_state_lemmas.
     model_state_interp tp δ -∗ has_fuels_S tid fs ==∗
     model_state_interp tp δ ∗ has_fuels tid fs.
   Proof.
-    iDestruct 1 as
-      (fm [Hfmle Hdom] Hfmdead Htp) "(Hδ & Hfm)".
+    iDestruct 1 as "(?&%fm&[%Hfmle%Hdom]&%Hfmdead&%Htp&Hδ & Hfm)".
     iIntros "Hfs".
     iDestruct (has_fuels_agree with "Hfm Hfs") as %Hagree.
     iMod (has_fuels_decr with "Hfm Hfs") as "[Hfm Hfs]".
     iModIntro. iFrame "Hfs".
-    iExists _. iFrame.
+    iSplit. iFrame. iExists _. iFrame.
     iPureIntro. repeat split.
     - eapply map_included_transitivity; [|done].
       rewrite -{2}(insert_id fm tid (S <$> fs)); [|done].
@@ -477,8 +482,7 @@ Section model_state_lemmas.
     { assert (delete ρ fs = fs) as ->.
       { apply delete_notin. by rewrite -not_elem_of_dom. }
       by iIntros "$$$". }
-    iDestruct 1 as
-      (fm [Hfmle Hdom] Hfmdead Htp) "(Hm & Hfm)".
+    iDestruct 1 as "(?&%fm&[%Hfmle%Hdom]&%Hfmdead&%Htp&Hm&Hfm)".
     iIntros "Hst Hfs".
     iDestruct (model_agree with "Hm Hst") as %Heq. rewrite !Heq.
     assert (is_Some (fs !! ρ)) as [f HSome].
@@ -486,7 +490,7 @@ Section model_state_lemmas.
     iDestruct (has_fuels_agree with "Hfm Hfs") as %Hagree.
     iMod (has_fuels_delete with "Hfm Hfs") as "[Hfm Hfs]".
     iModIntro.
-    iFrame "Hst". iFrame "Hfs".
+    iFrame "Hst". iFrame "Hfs". iSplit; first iFrame.
     iExists _. iFrame. rewrite Heq. iFrame.
     iPureIntro.
     repeat split; try done.
@@ -767,16 +771,20 @@ Section model_state_lemmas.
              (δ : LM) (ζ : locale Λ) (ρs : gset (fmrole M)) : LM :=
     model_update_decr ζ $ model_update_filter ζ ρs δ.
 
-  Lemma model_update_locale_spec extr (auxtr : auxiliary_trace LM) act ζ c2 ρs:
+  Lemma model_update_locale_spec extr (auxtr : auxiliary_trace LM) ζ c2 ρs:
+    valid_state_evolution_fairness extr auxtr →
     model_can_fuel_step (trace_last auxtr) ζ ((model_update_locale_fuel (trace_last auxtr) ζ) ρs) →
     tids_smaller c2.1 (model_update_locale_fuel (trace_last auxtr) ζ ρs) →
+    locale_step (trace_last extr) (inl (ζ, None)) c2 →
     valid_state_evolution_fairness
-      (extr :tr[inl (ζ, act)]: c2)
-      (auxtr :tr[Silent_step ζ act]:
+      (extr :tr[inl (ζ, None)]: c2)
+      (auxtr :tr[Silent_step ζ None]:
           (model_update_locale_fuel (trace_last auxtr) ζ) ρs).
   Proof.
-    intros Hstep Htids. destruct c2.
-    split; [done|]. split; [by apply model_can_fuel_step_trans|done].
+    intros Hvse Hstep Htids Hexstep. destruct c2 as [tp σ].
+    destruct Hvse as (?&?&?).
+    split; [| split]=>//.
+    econstructor=>//; first by apply model_can_fuel_step_trans.
   Qed.
 
   Definition map_disj (m : gmap (locale Λ) (gmap (fmrole M) nat)) :=
@@ -856,12 +864,12 @@ Section model_state_lemmas.
     set_solver.
   Qed.
 
-  Lemma model_state_interp_can_fuel_step es δ ζ fs :
+  Lemma model_state_interp_can_fuel_step es (δ : LiveState _ _) ζ fs :
     fs ≠ ∅ → model_state_interp es δ -∗ has_fuels_S ζ fs -∗
     ⌜model_can_fuel_step δ ζ ((model_update_locale_fuel δ ζ) (dom fs))⌝.
   Proof.
     iIntros (Hfs) "Hm Hfs".
-    iDestruct "Hm" as (fm Hfmle Hfmdead Htp) "(Hm & Hfm)".
+    iDestruct "Hm" as "(?&%fm&[%Hfmle%Hdom]&%Hfmdead&%Htp&Hm&Hfm)".
     rewrite /model_can_fuel_step.
     iDestruct (has_fuels_agree with "Hfm Hfs") as %Hagree.
     rewrite /fuel_map_le /fuel_map_le_inner map_included_spec in Hfmle.
@@ -972,7 +980,7 @@ Section model_state_lemmas.
     set_solver.
   Qed.
 
-  Lemma model_state_interp_fuel_update act c1 c2 δ ζ fs :
+  Lemma model_state_interp_fuel_update act c1 c2 (δ : LiveState _ _) ζ fs :
     locale_step c1 (inl (ζ, act)) c2 →
     model_state_interp c1.1 δ -∗
     has_fuels_S ζ fs ==∗
@@ -980,10 +988,10 @@ Section model_state_lemmas.
     has_fuels ζ fs.
   Proof.
     iIntros (Hstep) "Hm Hfs".
-    iDestruct "Hm" as (fm Hfmle Hfmdead Htp) "(Hm & Hfm)".
+    iDestruct "Hm" as "(?&%fm&[%Hfmle%Hdom]&%Hfmdead&%Htp&Hm&Hfm)".
     iDestruct (has_fuels_agree with "Hfm Hfs") as %Hagree.
     iMod (has_fuels_decr with "Hfm Hfs") as "[Hfm $]".
-    iModIntro. iExists _. iFrame. iPureIntro.
+    iModIntro. iSplit; first iFrame. iExists _. iFrame. iPureIntro.
     split; [|split].
     - by apply fuel_map_le_fuel_step.
     - by apply fuel_map_preserve_dead_fuel_step.
@@ -991,17 +999,18 @@ Section model_state_lemmas.
       apply elem_of_dom_2 in Hagree. by set_solver.
   Qed.
 
-  Lemma update_fuel_step extr (auxtr : auxiliary_trace LM) act c2 fs ζ :
+  Lemma update_fuel_step extr (auxtr : auxiliary_trace LM) c2 fs ζ :
     fs ≠ ∅ →
-    locale_step (trace_last extr) (inl (ζ, act)) c2 →
+    locale_step (trace_last extr) (inl (ζ, None)) c2 →
     has_fuels_S ζ fs -∗
+    ⌜ valid_state_evolution_fairness extr auxtr ⌝ -∗
     model_state_interp (trace_last extr).1 (trace_last auxtr) ==∗
     ∃ δ2,
       ⌜ valid_state_evolution_fairness
-        (extr :tr[inl (ζ, act)]: c2) (auxtr :tr[Silent_step ζ act]: δ2) ⌝ ∗
+        (extr :tr[inl (ζ, None)]: c2) (auxtr :tr[Silent_step ζ None]: δ2) ⌝ ∗
       has_fuels ζ fs ∗ model_state_interp c2.1 δ2.
   Proof.
-    iIntros (Hdom Hstep) "Hfuel Hm".
+    iIntros (Hdom Hstep) "Hfuel %Hvse Hm".
     iExists (model_update_locale_fuel (trace_last auxtr) ζ (dom fs)).
     iDestruct (model_state_interp_can_fuel_step with "Hm Hfuel") as %Hcan_step;
       [done|].
@@ -1010,7 +1019,7 @@ Section model_state_lemmas.
     iDestruct (model_state_interp_tids_smaller with "Hm") as %Htids.
     iModIntro.
     iFrame "Hm Hfuel".
-    iPureIntro. by apply model_update_locale_spec.
+    iPureIntro. apply model_update_locale_spec=>//.
   Qed.
 
   (** Model step *)
@@ -1118,7 +1127,7 @@ Section model_state_lemmas.
     frag_model_is s2.
   Proof.
     iIntros (Hfs Hlive Hstep Hmstep Hδ2) "Hm Hf Hs".
-    iDestruct "Hm" as (fm Hfmle Hfmdead Htp) "(Hm & Hfm)".
+    iDestruct "Hm" as "(?&%fm&%Hfmle&%Hfmdead&%Htp&Hm&Hfm)".
     iDestruct (has_fuels_agree with "Hfm Hf") as %Hagree.
     iMod (has_fuels_update _ _ _ ({[ρ := lm_fl LM s2]} ∪ fs) with "Hfm Hf")
       as "[Hfm Hf]".
@@ -1259,7 +1268,7 @@ Section model_state_lemmas.
     ⌜model_can_model_step δ ζ ρ δ2 fmact⌝.
   Proof.
     iIntros (Hstep Hle Hρ Hδ2) "Hm Hf Hδ".
-    iDestruct "Hm" as (fm Hfmle Hfmdead Htp) "(Hm & Hfm)".
+    iDestruct "Hm" as "(?&%fm&%Hfmle&%Hfmdead&%Htp&Hm&Hfm)".
     iDestruct (model_agree with "Hm Hδ") as %<-.
     iDestruct (has_fuels_agree with "Hfm Hf") as %Hagree.
     iPureIntro.
@@ -1339,13 +1348,16 @@ Section model_state_lemmas.
     (ls_data δ2) = model_update_model_step ζ ({[ρ]} ∪ ρs) ρ s2
                                            (trace_last auxtr) →
     model_can_model_step (trace_last auxtr) ζ ρ δ2 fmact →
+    valid_state_evolution_fairness extr auxtr →
     tids_smaller c2.1 δ2 →
     valid_state_evolution_fairness
       (extr :tr[inl (ζ, act)]: c2)
       (auxtr :tr[Take_step ρ fmact ζ act]: δ2).
   Proof.
-    intros Hstep Htids. destruct c2.
-    split; [done|]. split; [by apply model_can_model_step_trans|done].
+    intros Hstep Htids Hvse. destruct c2.
+    destruct Hvse as (?&?&?).
+    split; [| split]=>//.
+    econstructor=>//; first by apply model_can_model_step_trans.
   Qed.
 
   Lemma update_model_step
@@ -1357,6 +1369,7 @@ Section model_state_lemmas.
     locale_step (trace_last extr) (inl (ζ, act)) c2 →
     fmtrans _ s1 (inl (ρ, fmact)) s2 →
     has_fuels ζ ({[ρ := f]} ∪ (S <$> fs)) -∗ frag_model_is s1 -∗
+    ⌜valid_state_evolution_fairness extr auxtr⌝ -∗
     model_state_interp (trace_last extr).1 δ1 ==∗
     ∃ (δ2: LM),
       ⌜valid_state_evolution_fairness
@@ -1364,7 +1377,7 @@ Section model_state_lemmas.
       has_fuels ζ ({[ρ := LM.(lm_fl) s2]} ∪ fs) ∗
       frag_model_is s2 ∗ model_state_interp c2.1 δ2.
   Proof.
-    iIntros (Hlive Hdom Hlast Hstep Htrans) "Hfuel Hfrag Hm".
+    iIntros (Hlive Hdom Hlast Hstep Htrans) "Hfuel Hfrag %Hvse Hm".
     iDestruct (model_agree' with "Hm Hfrag") as %<-.
     pose proof (model_update_model_step_valid
                   ζ ({[ρ]} ∪ dom fs) ρ s2 δ1) as [δ2 Hδ2]; [done|].
@@ -1606,7 +1619,7 @@ Section model_state_lemmas.
     has_fuels (locale_of tp1 efork) fs2.
   Proof.
     iIntros (Hδ2 Hfs Hdisj Hforked Hstep) "Hm Hf".
-    iDestruct "Hm" as (fm Hfmle Hfmdead Htp) "(Hm & Hfm)".
+    iDestruct "Hm" as "(?&%fm&%Hfmle&%Hfmdead&%Htp&Hm&Hfm)".
     iDestruct (has_fuels_agree with "Hfm Hf") as %Hagree.
     assert (locale_of tp1 efork ∉ dom fm) as Hnin.
     { pose proof (not_elem_of_locale_of_from_list tp1 efork) as Hes%Htp.
@@ -1830,7 +1843,7 @@ Section model_state_lemmas.
     ⌜model_can_fork_step δ1 ζ (locale_of es e) δ2⌝.
   Proof.
     iIntros (Hδ2 Hne Hdisj) "Hm Hf".
-    iDestruct "Hm" as (fm [Hfmle Hdom] Hfmdead Htp) "(Hm & Hfm)".
+    iDestruct "Hm" as "(?&%fm&[%Hfmle %Hdom]&%Hfmdead&%Htp&Hm&Hfm)".
     iDestruct (has_fuels_agree with "Hfm Hf") as %Hagree.
     pose proof Hagree as Hagree'.
     rewrite /fuel_map_le_inner map_included_spec in Hfmle.
@@ -2005,17 +2018,20 @@ Section model_state_lemmas.
       apply not_elem_of_dom in Hes. set_solver.
   Qed.
 
-  Lemma model_update_locale_spec_fork act extr
+  Lemma model_update_locale_spec_fork extr
         (auxtr : auxiliary_trace LM) ζ ζf c2 ρs1 ρs2 δ2 :
+    valid_state_evolution_fairness extr auxtr →
     δ2.(ls_data) = model_update_fork ζ ζf ρs1 ρs2 (trace_last auxtr) →
     model_can_fork_step (trace_last auxtr) ζ ζf δ2 →
     tids_smaller c2.1 δ2 →
     valid_state_evolution_fairness
-      (extr :tr[inl (ζ, act)]: c2)
-      (auxtr :tr[Silent_step ζ act]: δ2).
+      (extr :tr[inl (ζ, None)]: c2)
+      (auxtr :tr[Silent_step ζ None]: δ2).
   Proof.
-    intros Hstep Htids. destruct c2.
-    split; [done|]. split; [by eapply model_can_fork_step_trans|done].
+    intros Hvse Hstep Htids. destruct c2.
+    destruct Hvse as (?&?&?).
+    split; [| split]=>//.
+    econstructor=>//; first by eapply model_can_fork_step_trans.
   Qed.
 
   Lemma model_state_interp_has_fuels_agree es δ ζ (fs : gmap (fmrole M) nat) :
@@ -2023,33 +2039,34 @@ Section model_state_lemmas.
     ⌜∃ fs', δ.(ls_map) !! ζ = Some fs' ∧ map_included (≤) fs fs'⌝.
   Proof.
     iIntros "Hm Hf".
-    iDestruct "Hm" as (fm [Hfmle _] Hfmdead Htp) "(Hm & Hfm)".
+    iDestruct "Hm" as "(?&%fm&[%Hfmle %Hdom]&%Hfmdead&%Htp&Hm&Hfm)".
     iDestruct (has_fuels_agree with "Hfm Hf") as %Hagree.
     rewrite /fuel_map_le_inner map_included_spec in Hfmle.
     apply Hfmle in Hagree as (fs'&HSome&Hfs').
     iPureIntro. by eexists _.
   Qed.
 
-  Lemma update_fork_step act fs1 fs2 tp1 tp2 (extr : execution_trace Λ)
+  Lemma update_fork_step fs1 fs2 tp1 tp2 (extr : execution_trace Λ)
         (auxtr: auxiliary_trace LM) ζ efork σ1 σ2 :
     fs1 ∪ fs2 ≠ ∅ → fs1 ##ₘ fs2 →
     trace_last extr = (tp1, σ1) →
-    locale_step (tp1, σ1) (inl (ζ, act)) (tp2, σ2) →
+    locale_step (tp1, σ1) (inl (ζ, None)) (tp2, σ2) →
+    valid_state_evolution_fairness extr auxtr →
     has_forked tp1 tp2 efork →
     has_fuels_S ζ (fs1 ∪ fs2) -∗
     model_state_interp tp1 (trace_last auxtr) ==∗
     ∃ δ2,
       ⌜valid_state_evolution_fairness
-        (extr :tr[inl (ζ, act)]: (tp2, σ2)) (auxtr :tr[Silent_step ζ act]: δ2)⌝ ∗
+        (extr :tr[inl (ζ, None)]: (tp2, σ2)) (auxtr :tr[Silent_step ζ None]: δ2)⌝ ∗
       has_fuels ζ fs1 ∗ has_fuels (locale_of tp1 efork) fs2 ∗
       model_state_interp tp2 δ2.
   Proof.
-    iIntros (Hdom Hdisj Hlast Hstep Hforked) "Hfuel Hm".
+    iIntros (Hdom Hdisj Hlast Hstep Hvse Hforked) "Hfuel Hm".
     iDestruct (model_state_interp_has_fuels_agree with "Hm Hfuel")
       as %(fs'&HSome&Hfs').
     iAssert (⌜(locale_of tp1 efork) ∉ dom (ls_map (trace_last auxtr))⌝)%I as %Hnin.
     { destruct Hforked as (?&?&?).
-      iDestruct "Hm" as (fm [_ Hdom'] _ Htp) "[Hm Hfm]".
+      iDestruct "Hm" as "(?&%fm&[%Hfmle %Hdom']&%Hfmdead&%Htp&Hm&Hfm)".
       rewrite -Hdom'.
       iPureIntro. apply not_elem_of_dom. apply Htp.
       apply locale_step_equiv in Hstep. simpl in *.
@@ -2100,5 +2117,15 @@ Section model_state_lemmas.
     - iModIntro. iFrame. iApply (own_proper with "Hfr2").
       do 2 f_equiv. set_solver.
   Qed.
+
+  (* Lemma update_model_state_interp_config (δ : LiveState _ _) cl fl tp m2 : *)
+  (*   LM.(lm_cfg_action) δ cl = (fl, m2) → *)
+  (*   ⊢ model_state_interp tp δ ==∗ model_state_interp tp {| ls_under := m2; ls_map := ls_map δ |}. *)
+  (* Proof. *)
+  (*   iIntros (Heq) "Hmod". unfold model_state_interp. *)
+  (*   iDestruct "Hmod" as (fm) "(#? & #? & #? & Hmod & Hfuel)". *)
+  (*   erewrite (lm_cfg_spec_live_roles) =>//. *)
+  (*   iExists fm. simpl. iFrame "Hfuel #". *)
+  (*   iMod (model_update _ _ m2 with "Hmod") as "[? ?]". *)
 
 End model_state_lemmas.
