fairneris/aneris_lang/state_interp/state_interp_config_wp.v
@@ -1,5 +1,6 @@
 From iris.proofmode Require Import tactics.
 From trillium.program_logic Require Export adequacy.
+From fairneris Require Import fuel.
 From fairneris.aneris_lang Require Import
      aneris_lang network resources.
 From fairneris.prelude Require Import gmultiset.
@@ -15,7 +16,6 @@ From fairneris.aneris_lang.state_interp Require Import
      state_interp_events
      state_interp_messages_history.
 From fairneris Require Import fairness.
-From fairneris.examples Require Import retransmit_model.
 
 From RecordUpdate Require Import RecordSet.
 Set Default Proof Using "Type".
@@ -24,7 +24,8 @@ Import uPred.
 Import RecordSetNotations.
 
 Section state_interpretation.
-  Context `{!anerisG retransmit_fair_model Σ}.
+  Context `{LM: LiveModel aneris_lang Mod}.
+  Context `{aG : !anerisG LM Σ}.
 
   (* TODO: Move this elsehwere and use it where we now use ad hoc induction *)
   Lemma fupd_elim_laterN E1 E2 n (P:iProp Σ) :
@@ -40,146 +41,135 @@ Section state_interpretation.
 
   (* OBS: A general update lemma could be nicer, but needs changes to
    [network_sockets_coh] API *)
-  Lemma state_buffers_insert ip (skts : gmap ip_address sockets)
-        sh skt bs m R Sn sa :
-    network_sockets_coh skts →
-    m_destination m = sa →
-    ip = ip_of_address sa →
-    skts !! ip = Some Sn →
-    Sn !! sh = Some (skt, R) →
-    saddress skt = Some sa →
-    model_state_socket_coh skts bs →
-    model_state_socket_coh (<[ip:=<[sh:=(skt, m :: R)]> Sn]> skts)
-                           (<[sa:=m :: R]> bs).
-  Proof.
-    intros Hscoh Hm -> Hip Hsh Hsa Hcoh ip' Sn' sh' skt' sa' R' Hip' Hsh' Hskt'.
-    assert (network_sockets_coh (<[ip_of_address sa:=<[sh:=(skt, m :: R)]> Sn]> skts)) as Hscoh'.
-    { by eapply network_sockets_coh_deliver_message. }
-    assert (ip_of_address sa' = ip') as <-.
-    { by eapply Hscoh'. }
-    destruct (decide (sa = sa')) as [<-|Hsaneq].
-    { destruct sa.
-      rewrite lookup_total_insert.
-      rewrite lookup_insert in Hip'.
-      simplify_eq.
-      assert(sh = sh') as <-.
-      { eapply Hscoh'; [| |done|..].
-        - apply lookup_insert.
-        - rewrite lookup_insert. done.
-        - done.
-        - rewrite Hsa. rewrite Hskt'. done. }
-      rewrite lookup_insert in Hsh'.
-      simplify_eq. done. }
-    rewrite lookup_total_insert_ne; [|done].
-    destruct (decide (ip_of_address sa = ip_of_address sa')) as [Heq|Hneq].
-    { rewrite Heq in Hip'. rewrite lookup_insert in Hip'.
-      simplify_eq.
-      assert(sh ≠ sh') as Hshneq.
-      { intros <-. rewrite lookup_insert in Hsh'. simplify_eq. }
-      rewrite lookup_insert_ne in Hsh'; [|done].
-      by eapply Hcoh. }
-    rewrite lookup_insert_ne in Hip'; [|done].
-    by eapply Hcoh.
-  Qed.
+  (* Lemma state_buffers_insert ip (skts : gmap ip_address sockets) *)
+  (*       sh skt bs m R Sn sa : *)
+  (*   network_sockets_coh skts → *)
+  (*   m_destination m = sa → *)
+  (*   ip = ip_of_address sa → *)
+  (*   skts !! ip = Some Sn → *)
+  (*   Sn !! sh = Some (skt, R) → *)
+  (*   saddress skt = Some sa → *)
+  (*   model_state_socket_coh skts bs → *)
+  (*   model_state_socket_coh (<[ip:=<[sh:=(skt, m :: R)]> Sn]> skts) *)
+  (*                          (<[sa:=m :: R]> bs). *)
+  (* Proof. *)
+  (*   intros Hscoh Hm -> Hip Hsh Hsa Hcoh ip' Sn' sh' skt' sa' R' Hip' Hsh' Hskt'. *)
+  (*   assert (network_sockets_coh (<[ip_of_address sa:=<[sh:=(skt, m :: R)]> Sn]> skts)) as Hscoh'. *)
+  (*   { by eapply network_sockets_coh_deliver_message. } *)
+  (*   assert (ip_of_address sa' = ip') as <-. *)
+  (*   { by eapply Hscoh'. } *)
+  (*   destruct (decide (sa = sa')) as [<-|Hsaneq]. *)
+  (*   { destruct sa. *)
+  (*     rewrite lookup_total_insert. *)
+  (*     rewrite lookup_insert in Hip'. *)
+  (*     simplify_eq. *)
+  (*     assert(sh = sh') as <-. *)
+  (*     { eapply Hscoh'; [| |done|..]. *)
+  (*       - apply lookup_insert. *)
+  (*       - rewrite lookup_insert. done. *)
+  (*       - done. *)
+  (*       - rewrite Hsa. rewrite Hskt'. done. } *)
+  (*     rewrite lookup_insert in Hsh'. *)
+  (*     simplify_eq. done. } *)
+  (*   rewrite lookup_total_insert_ne; [|done]. *)
+  (*   destruct (decide (ip_of_address sa = ip_of_address sa')) as [Heq|Hneq]. *)
+  (*   { rewrite Heq in Hip'. rewrite lookup_insert in Hip'. *)
+  (*     simplify_eq. *)
+  (*     assert(sh ≠ sh') as Hshneq. *)
+  (*     { intros <-. rewrite lookup_insert in Hsh'. simplify_eq. } *)
+  (*     rewrite lookup_insert_ne in Hsh'; [|done]. *)
+  (*     by eapply Hcoh. } *)
+  (*   rewrite lookup_insert_ne in Hip'; [|done]. *)
+  (*   by eapply Hcoh. *)
+  (* Qed. *)
 
-  Lemma state_buffers_delete ip (skts : gmap ip_address sockets)
-        sh skt bs m R Sn sa :
-    network_sockets_coh skts →
-    m_destination m = sa →
-    ip = ip_of_address sa →
-    skts !! ip = Some Sn →
-    Sn !! sh = Some (skt, R ++ [m]) →
-    saddress skt = Some sa →
-    model_state_socket_coh skts bs →
-    model_state_socket_coh (<[ip:=<[sh:=(skt, R)]> Sn]> skts)
-                           (<[sa:=R]> bs).
-  Proof.
-    intros Hscoh Hm -> Hip Hsh Hsa Hcoh ip' Sn' sh' skt' sa' R' Hip' Hsh' Hskt'.
-    assert (network_sockets_coh (<[ip_of_address sa:=<[sh:=(skt, R)]> Sn]> skts)) as Hscoh'.
-    { by eapply network_sockets_coh_receive. }
-    assert (ip_of_address sa' = ip') as <-.
-    { by eapply Hscoh'. }
-    destruct (decide (sa = sa')) as [<-|Hsaneq].
-    { destruct sa.
-      rewrite lookup_total_insert.
-      rewrite lookup_insert in Hip'.
-      simplify_eq.
-      assert(sh = sh') as <-.
-      { eapply Hscoh'; [| |done|..].
-        - apply lookup_insert.
-        - rewrite lookup_insert. done.
-        - done.
-        - rewrite Hsa. rewrite Hskt'. done. }
-      rewrite lookup_insert in Hsh'.
-      simplify_eq. done. }
-    rewrite lookup_total_insert_ne; [|done].
-    destruct (decide (ip_of_address sa = ip_of_address sa')) as [Heq|Hneq].
-    { rewrite Heq in Hip'. rewrite lookup_insert in Hip'.
-      simplify_eq.
-      assert(sh ≠ sh') as Hshneq.
-      { intros <-. rewrite lookup_insert in Hsh'. simplify_eq. }
-      rewrite lookup_insert_ne in Hsh'; [|done].
-      by eapply Hcoh. }
-    rewrite lookup_insert_ne in Hip'; [|done].
-    by eapply Hcoh.
-  Qed.
+  (* Lemma state_buffers_delete ip (skts : gmap ip_address sockets) *)
+  (*       sh skt bs m R Sn sa : *)
+  (*   network_sockets_coh skts → *)
+  (*   m_destination m = sa → *)
+  (*   ip = ip_of_address sa → *)
+  (*   skts !! ip = Some Sn → *)
+  (*   Sn !! sh = Some (skt, R ++ [m]) → *)
+  (*   saddress skt = Some sa → *)
+  (*   model_state_socket_coh skts bs → *)
+  (*   model_state_socket_coh (<[ip:=<[sh:=(skt, R)]> Sn]> skts) *)
+  (*                          (<[sa:=R]> bs). *)
+  (* Proof. *)
+  (*   intros Hscoh Hm -> Hip Hsh Hsa Hcoh ip' Sn' sh' skt' sa' R' Hip' Hsh' Hskt'. *)
+  (*   assert (network_sockets_coh (<[ip_of_address sa:=<[sh:=(skt, R)]> Sn]> skts)) as Hscoh'. *)
+  (*   { by eapply network_sockets_coh_receive. } *)
+  (*   assert (ip_of_address sa' = ip') as <-. *)
+  (*   { by eapply Hscoh'. } *)
+  (*   destruct (decide (sa = sa')) as [<-|Hsaneq]. *)
+  (*   { destruct sa. *)
+  (*     rewrite lookup_total_insert. *)
+  (*     rewrite lookup_insert in Hip'. *)
+  (*     simplify_eq. *)
+  (*     assert(sh = sh') as <-. *)
+  (*     { eapply Hscoh'; [| |done|..]. *)
+  (*       - apply lookup_insert. *)
+  (*       - rewrite lookup_insert. done. *)
+  (*       - done. *)
+  (*       - rewrite Hsa. rewrite Hskt'. done. } *)
+  (*     rewrite lookup_insert in Hsh'. *)
+  (*     simplify_eq. done. } *)
+  (*   rewrite lookup_total_insert_ne; [|done]. *)
+  (*   destruct (decide (ip_of_address sa = ip_of_address sa')) as [Heq|Hneq]. *)
+  (*   { rewrite Heq in Hip'. rewrite lookup_insert in Hip'. *)
+  (*     simplify_eq. *)
+  (*     assert(sh ≠ sh') as Hshneq. *)
+  (*     { intros <-. rewrite lookup_insert in Hsh'. simplify_eq. } *)
+  (*     rewrite lookup_insert_ne in Hsh'; [|done]. *)
+  (*     by eapply Hcoh. } *)
+  (*   rewrite lookup_insert_ne in Hip'; [|done]. *)
+  (*   by eapply Hcoh. *)
+  (* Qed. *)
 
+  (*TODO: lots of copy pasta! *)
   Lemma config_wp_correct : ⊢ config_wp.
   Proof.
     rewrite /config_wp. iModIntro.
     iIntros (ex atr c lbl σ2 Hexvalid Hex Hstep) "(% & Hsi & Hlive & Hauth)".
     rewrite (last_eq_trace_ends_in ex c); [|done].
+    rewrite /aneris_state_interp.
     iDestruct "Hsi" as (γm mh)
                          "(%Hhist & %Hgcoh & %Hnscoh & %Hmhcoh &
                            Hnauth & Hsi & Hlcoh & Hfreeips & Hmctx & Hmres)".
     iMod (steps_auth_update_S with "Hauth") as "Hauth".
     iApply fupd_elim_laterN; [solve_ndisj|].
     destruct c as [tp1 σ1]=> /=.
-    rewrite /simple_valid_state_evolution in H.
+    rewrite /valid_state_evolution_fairness in H.
     rewrite /trace_ends_in in Hex.
-    rewrite Hex in H. simpl in *.
+    have Hlstep: locale_step (tp1, σ1) (inr lbl) (tp1, σ2) by econstructor.
     destruct σ1; simpl in *; simplify_eq.
-    destruct (trace_last atr) as [[δ ms] bs] eqn:Hs.
+    pose (trace_last atr) as δ.
     inversion Hstep as
       [ip σ Sn Sn' sh a skt R m Hm HSn Hsh HSn' Hsaddr|
         σ|
         σ];
       simplify_eq/=.
     (* Deliver *)
-    - destruct H as (Hsteps & Hmatch & Hlive & Hσ).
-      iExists (δ, ms ∖ {[+ m +]}, <[m_destination m := m::R]>bs),
-                (inr ((), Some m)).
+    - destruct H as (Hsteps & Hmatch & Htids).
+      destruct (LM.(lm_cfg_action) (trace_last atr) (Some m)) as [ℓ δ'] eqn:Heq.
+      unshelve iExists ({| ls_data := {| ls_under := δ'; ls_map := δ.(ls_data).(ls_map) |} |}).
+      { admit. }
+      { admit. }
+      iExists (Config_step ℓ (Some m : config_label aneris_lang)).
       iSplitR.
       { iPureIntro.
-        rewrite /simple_valid_state_evolution.
+        rewrite /valid_state_evolution_fairness.
         rewrite /messages_to_receive_at_multi_soup in Hm.
         split.
-        { econstructor; [done|econstructor|done].
-          - destruct Hσ as [Hσ1 Hσ2].
-            simpl in *. rewrite Hσ1 in Hm.
-            apply elem_of_filter in Hm as [? Hm].
-            apply elem_of_gset_of_gmultiset in Hm.
-            set_solver.
-          - destruct Hσ as [Hσ1 Hσ2].
-            simpl in *.
-            assert (a = m_destination m) as ->.
-            { by apply elem_of_filter in Hm as [-> _]. }
-            by erewrite Hσ2. }
-        split; [done|].
-        split; [done|].
-        split.
-        { simpl. destruct Hσ as [Hσ1 Hσ2].
-          simpl in *. by rewrite Hσ1. }
-        simpl.
-        destruct Hσ as [Hσ1 Hσ2].
-        assert (a = m_destination m) as ->.
-        { by apply elem_of_filter in Hm as [-> _]. }
-        simpl in *.
-        apply state_buffers_insert; try done.
-        symmetry.
-        by eapply Hnscoh. }
-      iFrame "Hauth Hlive".
-      iModIntro.
+        { econstructor; [done|econstructor|done]; simpl.
+          - by eapply lm_cfg_spec_trans.
+          - split=>//. by eapply lm_cfg_spec_live_roles. }
+        split; first (split; [done|by eapply lm_cfg_spec_labels_match]).
+        by rewrite /tids_smaller ?Hex //= in Htids *. }
+      iFrame "Hauth". simpl.
+      iDestruct "Hlive" as "(#Hupd&%fm&?&?&?&Hst&?)".
+      iMod ("Hupd" $! _ _ _ _ Heq with "Hst").
+      iModIntro. iSplitL "Hnauth Hsi Hlcoh Hfreeips Hmctx Hmres"; last first.
+      { iSplit; iFrame "#". iExists fm. erewrite lm_cfg_spec_live_roles=>//. iFrame. }
       iExists γm, mh. iFrame.
       iSplit.
       { apply (last_eq_trace_ends_in) in Hex as ->.
@@ -193,24 +183,26 @@ Section state_interpretation.
       iSplitL "Hlcoh";
         [by iApply (local_state_coh_deliver_message with "Hlcoh")|].
       by iApply (free_ips_coh_deliver_message with "Hfreeips").
-    - destruct H as (Hsteps & Hmatch & Hlive & Hσ).
-      iExists (δ, ms ⊎ {[+ m +]}, bs), (inr ((), None)).
+    - destruct H as (Hsteps & Hmatch & Htids).
+      destruct (LM.(lm_cfg_action) (trace_last atr) None) as [ℓ δ'] eqn:Heq.
+      unshelve iExists ({| ls_data := {| ls_under := δ'; ls_map := δ.(ls_data).(ls_map) |} |}).
+      { admit. }
+      { admit. }
+      iExists (Config_step ℓ (None : config_label aneris_lang)).
       iSplitR.
       { iPureIntro.
-        rewrite /simple_valid_state_evolution.
+        rewrite /valid_state_evolution_fairness.
         split.
-        { econstructor; [done|econstructor|done].
-          destruct Hσ as [Hσ1 Hσ2].
-          simpl in *. by rewrite Hσ1 in H0. }
-        split; [done|].
-        split; [done|].
-        split.
-        { simpl. destruct Hσ as [Hσ1 Hσ2].
-          simpl in *. by rewrite Hσ1. }
-        simpl. by destruct Hσ as [Hσ1 Hσ2].
-      }
-      iFrame "Hauth Hlive".
-      iModIntro.
+        { econstructor; [done|econstructor|done]; simpl.
+          - by eapply lm_cfg_spec_trans.
+          - split=>//. by eapply lm_cfg_spec_live_roles. }
+        split; first (split; [done|by eapply lm_cfg_spec_labels_match]).
+        by rewrite /tids_smaller ?Hex //= in Htids *. }
+      iFrame "Hauth". simpl.
+      iDestruct "Hlive" as "(#Hupd&%fm&?&?&?&Hst&?)".
+      iMod ("Hupd" $! _ _ _ _ Heq with "Hst").
+      iModIntro. iSplitL "Hnauth Hsi Hlcoh Hfreeips Hmctx Hmres"; last first.
+      { iSplit; iFrame "#". iExists fm. erewrite lm_cfg_spec_live_roles=>//. iFrame. }
       iExists γm, mh. iFrame.
       iSplit.
       { apply (last_eq_trace_ends_in) in Hex as ->.
@@ -219,24 +211,26 @@ Section state_interpretation.
       iSplitR; [eauto using gnames_coh_update_sockets|].
       iSplitR; [eauto using network_sockets_coh_deliver_message|].
       eauto using messages_history_coh_duplicate_message.
-    - destruct H as (Hsteps & Hmatch & Hlive & Hσ).
-      iExists (δ, ms ∖ {[+ m +]}, bs), (inr ((), None)).
+    - destruct H as (Hsteps & Hmatch & Htids).
+      destruct (LM.(lm_cfg_action) (trace_last atr) None) as [ℓ δ'] eqn:Heq.
+      unshelve iExists ({| ls_data := {| ls_under := δ'; ls_map := δ.(ls_data).(ls_map) |} |}).
+      { admit. }
+      { admit. }
+      iExists (Config_step ℓ (None : config_label aneris_lang)).
       iSplitR.
       { iPureIntro.
-        rewrite /simple_valid_state_evolution.
+        rewrite /valid_state_evolution_fairness.
         split.
-        { econstructor; [done|econstructor|done].
-          destruct Hσ as [Hσ1 Hσ2].
-          simpl in *. by rewrite Hσ1 in H0. }
-        split; [done|].
-        split; [done|].
-        split.
-        { simpl. destruct Hσ as [Hσ1 Hσ2].
-          simpl in *. by rewrite Hσ1. }
-        simpl. by destruct Hσ as [Hσ1 Hσ2].
-      }
-      iFrame "Hauth Hlive".
-      iModIntro.
+        { econstructor; [done|econstructor|done]; simpl.
+          - by eapply lm_cfg_spec_trans.
+          - split=>//. by eapply lm_cfg_spec_live_roles. }
+        split; first (split; [done|by eapply lm_cfg_spec_labels_match]).
+        by rewrite /tids_smaller ?Hex //= in Htids *. }
+      iFrame "Hauth". simpl.
+      iDestruct "Hlive" as "(#Hupd&%fm&?&?&?&Hst&?)".
+      iMod ("Hupd" $! _ _ _ _ Heq with "Hst").
+      iModIntro. iSplitL "Hnauth Hsi Hlcoh Hfreeips Hmctx Hmres"; last first.
+      { iSplit; iFrame "#". iExists fm. erewrite lm_cfg_spec_live_roles=>//. iFrame. }
       iExists γm, mh. iFrame.
       iSplit.
       { apply (last_eq_trace_ends_in) in Hex as ->.
@@ -245,6 +239,6 @@ Section state_interpretation.
       iSplitR; [eauto using gnames_coh_update_sockets|].
       iSplitR; [eauto using network_sockets_coh_deliver_message|].
       eauto using messages_history_coh_drop_message.
-  Qed.
+  Admitted.
 
 End state_interpretation.
