fairneris/env_model.v
@@ -1,0 +1,78 @@
+From stdpp Require Import option countable.
+From fairneris Require Export inftraces trace_utils fairness.
+
+Record Lts lab `{Countable lab, Inhabited lab}: Type := {
+  lts_state :> Type;
+  lts_state_eqdec :: EqDecision lts_state;
+  lts_state_inhabited :: Inhabited lts_state;
+
+  lts_trans: lts_state → lab → lts_state → Prop;
+}.
+
+Arguments lts_state {_ _ _ _}.
+Arguments lts_trans {_ _ _ _}.
+
+Section models.
+  Context (Λ: language).
+  Context `{Countable (config_label Λ)}.
+  Context `{Countable (action Λ)}.
+  Context `{Inhabited (config_label Λ)}.
+  Context `{Inhabited (action Λ)}.
+
+Record EnvModel := {
+    env_lts :> Lts (action Λ + config_label Λ);
+    env_states_match : cfg Λ → env_lts.(lts_state) → Prop;
+    env_apply_trans : env_lts.(lts_state) → (action Λ + config_label Λ) → env_lts.(lts_state);
+    env_apply_trans_spec_both : ∀ ζ c1 m1 cl c2 m2,
+      env_apply_trans m1 cl = m2 →
+      locale_step c1 (sum_map (λ α, (ζ, Some α)) id cl) c2 →
+      env_states_match c1 m1 →
+      env_states_match c2 m2;
+    env_fairness: trace env_lts.(lts_state) (action Λ + config_label Λ) → Prop;
+}.
+
+Arguments env_lts {_}.
+
+Record UserModel := {
+    usr_role : Type;
+
+    usr_eqdec:: EqDecision usr_role;
+    usr_countable:: Countable usr_role;
+    usr_inhabited:: Inhabited usr_role;
+
+    usr_lts :> Lts (usr_role * option (action Λ));
+
+    usr_live_roles: usr_lts.(lts_state) → gset usr_role;
+    usr_live_spec: ∀ s ρ α s', usr_lts.(lts_trans) s (ρ,α) s' → ρ ∈ usr_live_roles s;
+}.
+
+Arguments usr_live_roles {_}.
+
+Inductive joint_trans {M: UserModel} {N: EnvModel} :
+  (M * N) → ((usr_role M * option (action Λ)) + config_label Λ) → (M * N) → Prop :=
+| UsrTrans n u1 u2 ρ : lts_trans M u1 (ρ, None) u2 → joint_trans (u1, n) (inl (ρ, None)) (u2, n)
+| NetTrans u n1 n2 ℓ : lts_trans N n1 (inr ℓ) n2 → joint_trans (u, n2) (inr ℓ) (u, n2)
+| SyncTrans u1 u2 n1 n2 ρ α :
+  lts_trans M u1 (ρ, Some α) u2 → lts_trans N n1 (inl α) n2 →
+  joint_trans (u1, n1) (inl (ρ, Some α)) (u2, n2)
+.
+
+Program Definition joint_model (M: UserModel) (N: EnvModel) : FairModel :=
+{|
+  fmstate := lts_state (usr_lts M) * lts_state N;
+  (* Why doesn't this work??? *)
+  fmrole := usr_role M;
+  fmaction := option (action Λ);
+  fmconfig := config_label Λ;
+  fmtrans s1 ℓ s2 := joint_trans s1 ℓ s2;
+  live_roles s := usr_live_roles s.1;
+
+  (* We want somehting like: *)
+  (* fmfairness tr := env_fairness _ tr; *)
+  (* but it's not so easy, because this definition is not constructive... *)
+  (* it may be easier to only state it on the joint model directly... *)
+  fmfairness _ := True;
+|}.
+Next Obligation. by intros ??????; inversion 1; simplify_eq; eapply usr_live_spec. Qed.
+
+End models.
