fairneris/testbed.v
@@ -1,0 +1,73 @@
+From stdpp Require Import option countable.
+From fairneris Require Export inftraces trace_utils fairness.
+
+Record Lts lab : Type := {
+  lts_state :> Type;
+  lts_state_eqdec :: EqDecision lts_state;
+  lts_state_inhabited :: Inhabited lts_state;
+
+  lts_lab_eqdec :: EqDecision lab;
+  lts_lab_countable : Countable lab;
+  lts_lab_inhabited :: Inhabited lab;
+
+  lts_trans: lts_state → lab → lts_state → Prop;
+}.
+
+Arguments lts_state {_}.
+Arguments lts_trans {_}.
+
+Record EnvModel (Λ : language) := {
+    env_lts :> Lts (action Λ + config_label Λ);
+    env_states_match : cfg Λ → env_lts.(lts_state) → Prop;
+    env_apply_trans : env_lts.(lts_state) → config_label Λ → env_lts.(lts_state);
+    env_apply_trans_spec : ∀ c1 m1 cl c2 m2,
+      env_apply_trans m1 cl = m2 →
+      locale_step c1 (inr cl) c2 →
+      env_states_match c1 m1 →
+      env_states_match c2 m2;
+}.
+
+Arguments env_lts {_}.
+
+Record UserModel (Λ : language) := {
+    usr_role : Type;
+    usr_lts :> Lts (usr_role * option (action Λ));
+
+    usr_eqdec: EqDecision usr_role;
+    usr_countable: Countable usr_role;
+    usr_inhabited: Inhabited usr_role;
+    usr_live_roles: usr_lts.(lts_state) → gset usr_role;
+    usr_live_spec: ∀ s ρ α s', usr_lts.(lts_trans) s (ρ,α) s' → ρ ∈ usr_live_roles s;
+}.
+
+Arguments usr_role {_}.
+Arguments usr_lts {_}.
+Arguments usr_live_roles {_ _}.
+
+Inductive joint_trans {Λ: language} {M: UserModel Λ} {N: EnvModel Λ} :
+  (M * N) → ((usr_role M * option (action Λ)) + config_label Λ) → (M * N) → Prop :=
+| UsrTrans n u1 u2 ρ : lts_trans M u1 (ρ, None) u2 → joint_trans (u1, n) (inl (ρ, None)) (u2, n)
+| NetTrans u n1 n2 ℓ : lts_trans N n1 (inr ℓ) n2 → joint_trans (u, n2) (inr ℓ) (u, n2)
+| SyncTrans u1 u2 n1 n2 ρ α :
+  lts_trans M u1 (ρ, Some α) u2 → lts_trans N n1 (inl α) n2 →
+  joint_trans (u1, n2) (inl (ρ, Some α)) (u2, n2)
+.
+
+Program Definition joint_model {Λ: language} (M: UserModel Λ) (N: EnvModel Λ) : FairModel :=
+{|
+  fmstate := lts_state (usr_lts M) * lts_state N;
+  (* Why doesn't this work??? *)
+  fmrole := usr_role M;
+  fmaction := option (action Λ);
+  fmconfig := config_label Λ;
+  fmtrans s1 ℓ s2 := joint_trans s1 ℓ s2;
+  live_roles s := usr_live_roles s.1;
+
+  fmrole_eqdec := usr_eqdec _ M;
+  fmrole_countable := usr_countable _ M;
+  fmrole_inhabited := usr_inhabited _ M;
+
+  (* let's see what to do later... *)
+  fmfairness _ := True;
+|}.
+Next Obligation. by intros ???????; inversion 1; simplify_eq; eapply usr_live_spec. Qed.
